06_Assembly.v
@@ -1,0 +1,54 @@
+(*  https://www.nand2tetris.org/project04  *)
+
+(* valid destination types. Is there a better way to factr this?
+All combinations of registers are possible.
+*)
+Inductive dest : Type :=
+| iNull | iM | iD | iMD | iA | iAM | iAD | iAMD.
+
+Inductive reg : Type :=
+| rA | rM | rD
+
+Inductive MA : Type :=
+| M | A
+(* M register is the location of RAM[A] *)
+(* A is an addressing register *)
+(* D is an actual register *)
+
+Inductive consts : Type :=
+| zero | one | negone
+
+Inductive comp : Type :=
+| cconst : consts -> comp (* fill with constant *)
+(* unary operations *)
+| creg : reg -> comp (* just put the register in the location *)
+| cnot : reg -> comp (* not of register *)
+| cneg : reg -> comp (* negative  of register *)
+| cinc : reg -> comp  (* increment of register *)
+| cdec : reg -> comp (* decrement register *)
+(* Binary operations always include D *)
+| cand : MA -> comp 
+| cor : MA -> comp 
+| cadd : MA -> comp
+| cDsub : MA -> comp (* D - A/M *)
+| csubD : MA -> comp. (* A/M - D *)
+
+
+Inductive jump : Type :=
+| JNull | JGT | JEQ | JGE | JLT | JNE | JLE | JMP.
+
+
+Inductive instr : Type := 
+| At : bits 15 -> instr
+| Comp : dest -> comp -> jump -> instr.
+
+
+
+Definition word := bits 16.
+Definition state := {rA : word, rD : word , ram : map addressspace word}
+
+Definition aeval (instate : state) (instr : instr) : state := 
+match instr with
+| At addr =>  instate (* setA state addr *)
+| Comp d c j => instate (* fill out the long implentation *)
+end. 
